cfrontend/BeeTypes.v
@@ -398,10 +398,15 @@ Definition ty_context := PTree.t type.
 
 (* To ensure that a location does not contain another location (ref) 
    and only points to basic types like int, bool, unit or pair *)
-Definition store_context := PTree.t type.  
+(* Records the type of the values that we expect to be stored in cell i *)
+Definition store_context := PTree.t basic_type.  
 
 Definition empty_context := (PTree.empty type).
 
 Definition extend_context (Gamma : ty_context) (k : ident) (t : type) := PTree.set k t Gamma. 
+
+Definition empty_stcontext := (PTree.empty basic_type).
+
+Definition extend_stcontext (Sigma : store_context) (k : ident) (t : basic_type) := PTree.set k t Sigma. 
 
 
